@prefix rdf: <http://www.w3.org/1999/02/22-rdf-syntax-ns#> .
@prefix xsd: <http://www.w3.org/2001/XMLSchema#> .
@prefix rdfs: <http://www.w3.org/2000/01/rdf-schema#> .
@prefix schema: <http://schema.org/> .
@prefix org: <http://www.w3.org/ns/org#> .
@prefix foaf: <http://xmlns.com/foaf/0.1/> .
@prefix parking: <http://data.gmdsp.org.uk/def/council/parking/> .

#################################################################
#
#    Classes
#
#################################################################

parking:ParkingSite
      rdfs:label "Parking site"^^xsd:string ;
      rdfs:subClassOf schema:ParkingFacility ;
      rdfs:isDefinedBy <http://data.gmdsp.org.uk/def/council/parking> .

parking:ParkingSiteOperator
      rdfs:label "Parking site operator"^^xsd:string ;
      rdfs:subClassOf org:Organization ;
      rdfs:isDefinedBy <http://data.gmdsp.org.uk/def/council/parking> .

#################################################################
#
#    Properties
#
#################################################################

parking:operator
      	rdf:type rdf:Property ;
      	rdfs:label "Car park operator"^^xsd:string ;
	  	rdfs:comment "The organisation responsible for operating a particular car park" ;
      	rdfs:domain parking:ParkingSiteOperator ;
 	rdfs:range xsd:string .

parking:totalNumberOfSpaces
      rdf:type rdf:Property ;
      rdfs:label "Total number of spaces"^^xsd:string ;
		rdfs:comment "The total number of parking spaces in a particular car park" ;
      rdfs:domain parking:ParkingSite ;      
      rdfs:range xsd:integer .

parking:totalNumberOfDisabledSpaces
      rdf:type rdf:Property ;
      rdfs:label "Total number of spaces"^^xsd:string ;
		rdfs:comment "The total number of disabled parking spaces in a particular car park" ;
      rdfs:domain parking:ParkingSite ;
      rdfs:range xsd:integer .

parking:totalNumberOfFreeSpaces
      rdf:type rdf:Property ;
      rdfs:label "Total number of spaces"^^xsd:string ;
		rdfs:comment "The total number of free parking spaces in a particular car park" ;
      rdfs:domain <http://data.gmdsp.org.uk/def/council/parking/ParkingSite> ;
      rdfs:range xsd:integer .

parking:totalNumberOfChargableSpaces
      rdf:type rdf:Property ;
      rdfs:label "Total number of spaces"^^xsd:string ;
		rdfs:comment "The total number of chargeable parking spaces in a particular car park" ;
      rdfs:domain parking:ParkingSite ;
      rdfs:range xsd:integer .

parking:totalNumberOfInfoPoints
      rdf:type rdf:Property ;
      rdfs:label "Total number of spaces"^^xsd:string ;
		rdfs:comment "The total number of information points in a particular car park" ;
      rdfs:domain parking:ParkingSite ;
      rdfs:range xsd:integer .

parking:totalNumberOfMachines
      rdf:type rdf:Property ;
      rdfs:label "Total number of spaces"^^xsd:string ;
		rdfs:comment "The total number of payment machines in a particular car park" ;
      rdfs:domain parking:ParkingSite ;
      rdfs:range xsd:integer .

parking:totalNumberOfCCTVCameras
      rdf:type rdf:Property ;
      rdfs:label "Total number of spaces"^^xsd:string ;
      		rdfs:comment "The total number of CCTV cameras in a particular car park" ;
      rdfs:domain parking:ParkingSite ;
      rdfs:range xsd:integer .

parking:electricVehicleChargingPoint
      rdf:type rdf:Property ;
      rdfs:label "Electric vehicle charging point"^^xsd:string ;
	      rdfs:comment "Does the car park have charging points for electric vehicles?" ;
      rdfs:domain parking:ParkingSite ;
      rdfs:range xsd:string .
      
parking:informationPage
        rdf:type rdf:Property ;
        rdfs:label "Information page"^^xsd:string ;
        	rdfs:comment "Page (given by URL) with information for this parking site."^^xsd:string ;
      	rdfs:domain parking:ParkingSite ;
        rdfs:subPropertyOf foaf:page .

parking:parkingType
        rdf:type rdf:Property ;
        rdfs:label "Parking type"^^xsd:string ;
        	rdfs:comment "The type of parking site eg. pay and display"^^xsd:string ;
      	rdfs:domain parking:ParkingSite ;
 	rdfs:range xsd:string .

parking:barrierType
        rdf:type rdf:Property ;
        rdfs:label "Barrier type"^^xsd:string ;
        	rdfs:comment "The type of barrier at the parking site."^^xsd:string ;
      	rdfs:domain parking:ParkingSite ;
 	rdfs:range xsd:string .
 	
 parking:chargingCategory
        rdf:type rdf:Property ;
        rdfs:label "Charging category type"^^xsd:string ;
        	rdfs:comment "The charging category in operation at the parking site."^^xsd:string ;
      	rdfs:domain parking:ParkingSite ;
 	rdfs:range xsd:string .	
  	
 parking:heightRestriction
        rdf:type rdf:Property ;
        rdfs:label "Height restriction"^^xsd:string ;
        	rdfs:comment "The height restriction in operation at the parking site."^^xsd:string ;
      	rdfs:domain parking:ParkingSite ;
 	rdfs:range xsd:string .		
